decidabilityScript.sml
@@ -27,8 +27,8 @@ Define `okPfx g p = ?sfx.(p++sfx) IN (language g)`
 
 val maxPfx = Define
 `maxPfx g p s = ?sf.okPfx g p /\ (p++sf = s)
-	    /\ (!p'.IS_PREFIX p' p ==> 
-	         (p=p') \/ ~okPfx g p'`
+	         /\ (!p'.IS_PREFIX p' p ==> 
+	                (p=p') \/ ~okPfx g p')`
 
 val maxPfxExists =
 store_thm ("maxPfxExists",
@@ -37,6 +37,39 @@ store_thm ("maxPfxExists",
 !s.?pfx sfx sfx'.maxPfx g pfx s /\ (s=pfx++sfx)
 /\ (pfx++sfx') IN (language ag)``,
 MAGIC)
+
+
+``(pfx++sfx) IN language g ==>
+  ?p p'.(pfx=p++p') /\
+  ?rst rhs lhs.handleg g pfx rhs (p',lhs,rst)``
+SRW_TAC [] [language_def] THEN
+FULL_SIMP_TAC (srw_ss()) [Once RTC_CASES2] 
+THENL[
+      MAGIC,
+
+      FULL_SIMP_TAC (srw_ss()) [derives_def] THEN
+      SRW_TAC [] [] THEN
+      `(s1++rhs = pfx) /\ (s2 = sfx) \/
+       (?s1' s2'.
+          (s1++rhs = pfx ++ s1') /\ (s2 = s2') /\
+          (sfx = s1' ++ s2')) \/
+       ?s1' s2'.
+         (pfx = s1++rhs ++ s1') /\ (sfx = s2') 
+       /\ (s2 = s1' ++ s2')`
+	  by METIS_TAC [twoListAppEq] THEN
+      SRW_TAC [][]
+      THENL[
+
+	    SRW_TAC [] [handleg_def]
+
+]
+
+
+
+``(auggr g st eof = SOME m) ==>
+  (slr ag = SOME m) ==>
+  (!nt. nt IN nonTerminals ag ==> gaw ag nt) ==>
+    ``
 
 
 
